Fix mod ops (leq comparison)

code/experimental/rsapss/Hacl.Impl.Bignum.Comparison.fst
@@ -12,26 +12,31 @@ open Lib.Buffer
 open Hacl.Impl.Bignum.Convert
 open Hacl.Impl.Bignum.Core
 
-val bn_is_less_:
+
+val max': a:size_t -> b:size_t -> size_t
+let max' a b = if a >=. b then a else b
+
+val bn_compare_generic:
      #aLen:bn_len
-  -> #bLen:bn_len{v bLen <= v aLen}
+  -> #bLen:bn_len
   -> a:lbignum aLen
   -> b:lbignum bLen
   -> finval:bool
-  -> i:size_t{v i <= v aLen}
+  -> i:size_t
   -> Stack bool
     (requires fun h -> live h a /\ live h b)
     (ensures  fun h0 _ h1 -> modifies loc_none h0 h1 /\ h0 == h1)
-let rec bn_is_less_ #aLen #bLen a b finval i =
+let rec bn_compare_generic #aLen #bLen a b finval i =
   if i =. 0ul then finval else begin
     let i = i -. size 1 in
-    let t1 = a.(i) in
+    let t1 = bval aLen a i in
     let t2 = bval bLen b i in
     (if not (eq_u64 t1 t2) then
       if lt_u64 t1 t2 then true else false
-    else bn_is_less_ a b finval i)
+    else bn_compare_generic a b finval i)
   end
 
+inline_for_extraction
 val bn_is_less:
      #aLen:bn_len
   -> #bLen:bn_len
@@ -42,15 +47,13 @@ val bn_is_less:
     (ensures  fun h0 r h1 ->
      modifies loc_none h0 h1 /\ h0 == h1 /\
      r == (as_snat h0 a < as_snat h0 b))
-[@"c_inline"]
 let bn_is_less #aLen #bLen a b =
-    let res =
-      if bLen <=. aLen
-      then (assert (v bLen <= v aLen); bn_is_less_ #aLen #bLen a b false aLen)
-      else (let res = bn_is_less_ #bLen #aLen b a false bLen in not res) in
-    admit();
-    res
+  let res = bn_compare_generic a b false (max' aLen bLen) in
+  let h = FStar.HyperStack.ST.get () in
+  assume (res == (as_snat h a < as_snat h b));
+  res
 
+inline_for_extraction
 val bn_is_leq:
      #aLen:bn_len
   -> #bLen:bn_len
@@ -61,28 +64,25 @@ val bn_is_leq:
     (ensures  fun h0 r h1 ->
      modifies loc_none h0 h1 /\ h0 == h1 /\
      r == (as_snat h0 a <= as_snat h0 b))
-[@"c_inline"]
 let bn_is_leq #aLen #bLen a b =
-    let res =
-      if bLen <=. aLen
-      then (assert (v bLen <= v aLen); bn_is_less_ #aLen #bLen a b true aLen)
-      else (let res = bn_is_less_ #bLen #aLen b a true bLen in not res) in
-    admit();
-    res
+  let res = bn_compare_generic a b true (max' aLen bLen) in
+  let h = FStar.HyperStack.ST.get () in
+  assume (res == (as_snat h a <= as_snat h b));
+  res
 
 val bn_is_equal_:
      #aLen:bn_len
-  -> #bLen:bn_len{v bLen <= v aLen}
+  -> #bLen:bn_len
   -> a:lbignum aLen
   -> b:lbignum bLen
-  -> i:size_t{v i <= v aLen}
+  -> i:size_t
   -> Stack bool
     (requires fun h -> live h a /\ live h b)
     (ensures  fun h0 _ h1 -> modifies loc_none h0 h1 /\ h0 == h1)
 let rec bn_is_equal_ #aLen #bLen a b i =
   if i >. 0ul then
     let i = i -. size 1 in
-    let t1 = a.(i) in
+    let t1 = bval aLen a i in
     let t2 = bval bLen b i in
     (if not (eq_u64 t1 t2) then false else bn_is_equal_ a b i)
   else true
@@ -100,13 +100,12 @@ val bn_is_equal:
      modifies loc_none h0 h1 /\ h0 == h1 /\
      r == (as_snat h0 a = as_snat h0 b))
 let bn_is_equal #aLen #bLen a b =
-    let res =
-      if bLen <=. aLen
-      then (bn_is_equal_ #aLen #bLen a b aLen)
-      else (bn_is_equal_ #bLen #aLen b a bLen) in
-    admit();
-    res
+  let res = bn_is_equal_ a b (max' aLen bLen) in
+  let h = FStar.HyperStack.ST.get () in
+  assume (res == (as_snat h a = as_snat h b));
+  res
 
+inline_for_extraction
 val bn_is_greater:
      #aLen:bn_len
   -> #bLen:bn_len
@@ -117,9 +116,9 @@ val bn_is_greater:
     (ensures  fun h0 r h1 ->
      modifies loc_none h0 h1 /\ h0 == h1 /\
      r == (as_snat h0 a > as_snat h0 b))
-[@"c_inline"]
 let bn_is_greater #aLen #bLen a b = bn_is_less b a
 
+inline_for_extraction
 val bn_is_geq:
      #aLen:bn_len
   -> #bLen:bn_len
@@ -130,5 +129,4 @@ val bn_is_geq:
     (ensures  fun h0 r h1 ->
      modifies loc_none h0 h1 /\ h0 == h1 /\
      r == (as_snat h0 a >= as_snat h0 b))
-[@"c_inline"]
 let bn_is_geq #aLen #bLen a b = bn_is_leq b a
